Add basic TM simulator

regex-new.dfy
@@ -621,3 +621,159 @@ ensures forall tape: HalfTape :: half_tape_matches(tape, r) ==> exists cover :: 
 
   return { r };
 }
+
+/// The TM step goes here
+
+// 'cons' adds a bit to the beginning of the provided tape.
+// Adding zero to the beginning of an empty tape does nothing.
+function method cons(b: Bit, t: HalfTape): HalfTape {
+  if b == B0 && t == HalfTape([])
+    then HalfTape([])
+    else
+      var result := [b] + t.initial;
+      assert result[|result|-1] != B0;
+      HalfTape(result)
+}
+
+function method tail(t: HalfTape): HalfTape {
+  if t == HalfTape([]) then HalfTape([]) else HalfTape(t.initial[1..])
+}
+
+function method head(t: HalfTape): Bit {
+  if t == HalfTape([]) then B0 else t.initial[0]
+}
+
+// This lemma verifies that cons and uncons are "opposites", so that adding
+// and then removing a bit leaves the tape in its initial state,
+// and that removing and then adding back a bit leaves the tape in its
+// initial state.
+//
+// This lemma is not actually used below, since Dafny can prove it automatically.
+lemma cons_uncons(tape: HalfTape)
+ensures tail(cons(B0, tape)) == tape
+ensures tail(cons(B1, tape)) == tape
+ensures cons(head(tape), tail(tape)) == tape {
+}
+
+// Because the word "state" would otherwise be overloaded, the 5 "states" for the
+// TM are instead called "Colors": CA, CB, CC, CD, CE, with the "C" standing for "Color".
+datatype Color = CA | CB | CC | CD | CE
+
+// A machine state describes the machine's color and the tape that it finds itself in.
+// Conceptually, the machine head is over the "head_symbol" bit and about to process that
+// bit. The `left` and `right` fields describe the half-infinite tape to the left of the
+// head and to the right.
+//
+// Note that this representation avoids explicitly representing the TM's location in space.
+// This simplifies the logic and presentation below.
+datatype MachineState = MachineState(color: Color, head_symbol: Bit, left: HalfTape, right: HalfTape)
+
+// The TM can move left or right at each step.
+datatype Direction = L | R
+
+// An action describes what the machine might be told to do by a program:
+// - write the given bit
+// - switch to the given color
+// - move one step in given direction
+datatype Action = Action(write: Bit, new_color: Color, move: Direction)
+
+// machine_step_action applies the given action to the machine state.
+function method machine_step_action(m: MachineState, action: Action): MachineState {
+  match action.move {
+    case L => MachineState(
+      // The new color comes from the action.
+      color := action.new_color,
+      // The next symbol to be read comes from the first symbol in the left tape.
+      head_symbol := head(m.left),
+      // We remove one symbol from the left tape.
+      left := tail(m.left),
+      // The written bit ends up at the beginning of the right tape.
+      right := cons(action.write, m.right)
+    )
+    // This case is identical to the case above, but with left/right reversed.
+    case R => MachineState(
+      // The new color comes from the action.
+      color := action.new_color,
+      // The next symbol to be read comes from the first symbol in the right tape.
+      head_symbol := head(m.right),
+      // We remove one symbol from the right tape.
+      right := tail(m.right),
+      // The written bit ends up at the beginning of the left tape.
+      left := cons(action.write, m.left)
+    )
+  }
+}
+
+// All TMs are assumed to begin in the color CA, on a tape of all zeros.
+const initial: MachineState := MachineState(Color.CA, Bit.B0, HalfTape([]), HalfTape([]))
+
+// `ProgramStepInput` is a structure containing the information needed to find out what
+// action should be applied next in a TM program.
+datatype ProgramStepInput = ProgramStepInput(head: Bit, color: Color)
+
+// A program is a (partial) mapping from inputs to actions, describing what the TM
+// should do next in each situation.
+//
+// If a transition is absent, then it is assumed to be a halting transition.
+type Program = map<ProgramStepInput, Action>
+
+// A `MachineStep` either is either `Halt` if no transition for the current state
+// exists, or it is NextMachine and holds that next state.
+datatype MachineStep = NextMachine(next_state: MachineState) | Halt
+
+// machine_step causes the provided state to step forward once according to the
+// provided program. The output will either be the next state, or Halt if there
+// is no configured transition.
+function method machine_step(program: Program, m: MachineState): MachineStep {
+  if ProgramStepInput(m.head_symbol, m.color) in program
+    then NextMachine(machine_step_action(m, program[ProgramStepInput(m.head_symbol, m.color)]))
+    else Halt
+}
+
+// This function is a helper for moving 'n' steps forward in time.
+// It is a `function` rather than `function method` because it will cause stack-overflow if run
+// for more than a small number of iterations.
+function machine_step_n(program: Program, m: MachineState, n: nat): MachineStep {
+  if n == 0
+    // If n is zero, then the output is the same as the initial program.
+    then NextMachine(m)
+    // Otherwise, run n-1 steps. If that machine has not yet halted, run it one
+    // more step.
+    else match machine_step_n(program, m, n-1) {
+      case Halt => Halt
+      case NextMachine(m2) => machine_step(program, m2)
+    }
+}
+
+// This method computes the same value as `machine_step_n` (guaranteed by its ensures clause below).
+// This version can be called at runtime because it will not overflow the stack.
+method machine_step_iterative(program: Program, m: MachineState, n: nat)
+returns (result: MachineStep)
+ensures result == machine_step_n(program, m, n) {
+  var i := 0;
+  var current_state := NextMachine(m);
+
+  while i < n
+  invariant 0 <= i <= n
+  invariant current_state == machine_step_n(program, m, i)
+  {
+    current_state := if current_state.Halt? then Halt else machine_step(program, current_state.next_state);
+    i := i + 1;
+  }
+  return current_state;
+}
+
+// This function returns the nth TM state for a program, starting from the
+// initial state.
+function machine_iter_n(program: Program, n: nat): MachineStep {
+  machine_step_n(program, initial, n)
+}
+
+// By definition, a machine halts if there's a step such that at that point, it halts.
+predicate program_eventually_halts(program: Program) {
+  exists n :: n >= 0 && machine_iter_n(program, n).Halt?
+}
+
+predicate program_loops_forever(program: Program) {
+  !program_eventually_halts(program)
+}
